changed dominators tree construction algorithms.
step 1) for each node n, sort all its strict dominators, then we get a
chain of dominators (from the entry to n)
step 2) from a tree with only one node - entry, we insert leaves by
traversing each sorted chains.

The old algorithm is
1) generating immediate dominators for each node
2) generating a list of edges sorted by the partial order imposed by 1)
3) construting a graph-theory tree by adding edges in the order of 2)
4) converting 3) to a inductive tree we wanted.

The old algorithm is 
1) slow because
   a) 3)4) can be done in one step in fact
   b) we do not keep the order information for each pair from step 1), and have
      to restruct them at step 2)
2) hard to prove, because there are many invariant to check, and 3) is designed 
   by Program Fixpoint.
3) Coq extraction does not eliminate all computation-irrevalent code,
   because some invariant was designed by Type... which makes programs
   slow.

The new algorithm can be designed by simple structural Fixpoint,
reduced 1/3 compilation time, too.



git-svn-id: https://webdav.seas.upenn.edu/svn/sol/vol@3390 eef5ea85-cc2e-0410-bd84-0fae1f012da8

src/Transforms/dtree.v
@@ -50,14 +50,20 @@ Proof.
 Qed.
 
 Lemma remove_neq_in': forall (a b:A) (l1: list A),
-  a <> b ->
   In a (List.remove Hdec b l1) ->
-  In a l1.
+  In a l1 /\ a <> b.
 Proof.
   induction l1; simpl; intros; auto.
-    destruct (Hdec b a0); subst; simpl; auto.
-      simpl in H0.
-      destruct H0 as [H0 | H0]; subst; auto.
+    destruct (Hdec b a0); subst; simpl.
+      apply IHl1 in H.
+      destruct H as [H1 H2].
+      split; auto.
+
+      simpl in H.
+      destruct H as [H | H]; subst; auto.
+      apply IHl1 in H.
+      destruct H as [H1 H2].
+      split; auto.
 Qed.
 
 End MoreMove.
@@ -164,6 +170,346 @@ with WF_dtrees (f:fdef) : l -> DTrees -> Prop :=
              WF_dtrees f l0 (DT_cons dt0 dts0)
 .
 
+(* l1 >> l2, l1 strict dominates l2 *)
+Definition gt_sdom (res: AMap.t (set l)) (l1 l2:l) : bool :=
+match AMap.get l2 res with
+| dts2 => in_dec l_dec l1 dts2
+end.
+
+Fixpoint find_min (res: AMap.t (set l)) (acc:l) (dts: set l): l :=
+match dts with
+| nil => acc
+| l0::dts' =>
+    if (gt_sdom res acc l0) then
+      find_min res l0 dts' 
+    else
+      find_min res acc dts' 
+end.
+
+Fixpoint insert_sdom_iter (res: AMap.t (set l)) (l0:l) (prefix suffix:list l) 
+  : list l :=
+match suffix with
+| nil => List.rev (l0 :: prefix)
+| l1::suffix' => 
+    if gt_sdom res l0 l1 then (List.rev (l0 :: prefix)) ++ suffix
+    else insert_sdom_iter res l0 (l1::prefix) suffix'
+end.
+
+Fixpoint insert_sort_sdom (res: AMap.t (set l)) (data:list l) (acc:list l) 
+  : list l :=
+match data with
+| nil => acc 
+| l1 :: data' => insert_sort_sdom res data' (insert_sdom_iter res l1 nil acc)
+end.
+
+Definition sort_sdom (res: AMap.t (set l)) (data:list l) : list l :=
+insert_sort_sdom res data nil.
+
+Require Import Sorted.
+
+Definition gt_sdom_prop (res: AMap.t (set l)) (l1 l2:l) : Prop :=
+gt_sdom res l1 l2 = true.
+
+Lemma insert_sdom_iter_sorted: forall res input,
+  Sorted (gt_sdom_prop res) (sort_sdom res input).
+Admitted.
+
+Lemma insert_sdom_iter_safe: forall res input l0,
+  In l0 input <-> In l0 (sort_sdom res input).
+Admitted.
+
+Fixpoint remove_redundant (input: list l) : list l :=
+match input with
+| a :: ((b :: _) as input') =>
+    if (l_dec a b) then remove_redundant input'
+    else a :: remove_redundant input'
+| _ => input
+end.
+
+Lemma remove_redundant_safe: forall input l0,
+  In l0 input <-> In l0 (remove_redundant input).
+Admitted.
+
+Lemma remove_redundant_sorted: forall R input,
+  Sorted R input ->
+  Sorted R (remove_redundant input) /\ NoDup (remove_redundant input).
+Admitted.
+
+Fixpoint compute_sdom_chains_aux (res: AMap.t (set l)) (bd: list l) 
+  (acc: list (l * list l)) : list (l * list l) :=
+match bd with
+| nil => acc
+| l0 :: bd' => 
+    compute_sdom_chains_aux res bd' 
+      ((l0, remove_redundant (sort_sdom res (l0 :: AMap.get l0 res)))::acc)
+end.
+
+Definition compute_sdom_chains (res: AMap.t (set l)) (bd: list l) 
+  : list (l * list l) :=
+compute_sdom_chains_aux res bd nil.
+
+Lemma compute_sdom_chains_sorted: forall res bd l0 chain,
+  In (l0, chain) (compute_sdom_chains res bd) ->
+  Sorted (gt_sdom_prop res) chain /\ NoDup chain.
+Admitted.
+
+Lemma compute_sdom_chains_safe: forall res bd l0 chain l1,
+  In (l0, chain) (compute_sdom_chains res bd) ->
+  (In l1 chain <-> In l1 (l0 :: AMap.get l0 res)).
+Admitted.
+
+Fixpoint dep_doms__nondep_doms_aux bd0 (res: AMap.t (Dominators.t bd0)) 
+  bd (acc: AMap.t (set l)) : AMap.t (set l) :=
+match bd with
+| nil => acc
+| l0::bd' => 
+    match AMap.get l0 res with
+    | (Dominators.mkBoundedSet dts0 _) =>
+        AMap.set l0 dts0 (dep_doms__nondep_doms_aux bd0 res bd' acc)
+    end
+end.
+
+Definition dep_doms__nondep_doms bd (res: AMap.t (Dominators.t bd)) 
+  : AMap.t (set l) :=
+dep_doms__nondep_doms_aux bd res bd (AMap.init nil).
+
+Definition wf_chain f dt (chain:list l) : Prop :=
+match chain with
+| entry :: _ => 
+   let b := bound_fdef f in
+   let res := dep_doms__nondep_doms b (dom_analyze f) in
+   entry `in` dtree_dom dt /\
+   NoDup chain /\ Sorted (gt_sdom_prop res) chain
+| _ => True
+end.
+
+Definition getEntryLabel (f:fdef) : option l :=
+match f with
+| fdef_intro _ ((block_intro l0 _ _ _)::_) => Some l0
+| _ => None
+end.
+
+Lemma compute_sdom_chains__wf_chain: forall f l0 chain0 entry rd,
+  getEntryLabel f = Some entry ->
+  reachablity_analysis f =  Some rd ->
+  In (l0, chain0)
+    (compute_sdom_chains
+       (dep_doms__nondep_doms (bound_fdef f) (dom_analyze f)) rd) ->
+  wf_chain f (DT_node entry DT_nil) chain0.
+Admitted.
+
+Fixpoint in_children_roots child dts : bool :=
+match dts with
+| DT_nil => false
+| DT_cons (DT_node l0 _) dts' =>
+    if (l_dec l0 child) then true else in_children_roots child dts'
+end.
+
+Fixpoint dtree_insert dt parent child : DTree :=
+match dt with
+| DT_node l0 dts0 => 
+    if (id_dec parent l0) then 
+      if in_children_roots child dts0 then dt
+      else DT_node l0 (DT_cons (DT_node child DT_nil) dts0)
+    else DT_node l0 (dtrees_insert dts0 parent child)
+end
+with dtrees_insert (dts: DTrees) parent child : DTrees :=
+match dts with
+| DT_nil => DT_nil
+| DT_cons dt0 dts0 => 
+    DT_cons (dtree_insert dt0 parent child) (dtrees_insert dts0 parent child)
+end.
+
+Fixpoint is_dtree_edge dt parent child : bool :=
+match dt with
+| DT_node l0 dts0 => 
+    if (id_dec parent l0) then 
+      if in_children_roots child dts0 then true
+      else is_dtrees_edge dts0 parent child
+    else is_dtrees_edge dts0 parent child
+end
+with is_dtrees_edge (dts: DTrees) parent child : bool :=
+match dts with
+| DT_nil => false
+| DT_cons dt0 dts0 => 
+    is_dtree_edge dt0 parent child || is_dtrees_edge dts0 parent child
+end.
+
+Scheme dtree_rec2 := Induction for DTree Sort Set
+  with dtrees_rec2 := Induction for DTrees Sort Set.
+
+Definition dtree_mutrec P P' :=
+  fun h1 h2 h3 => 
+    (pair (@dtree_rec2 P P' h1 h2 h3) (@dtrees_rec2 P P' h1 h2 h3)).
+
+Definition dtree_insert__wf_dtree_prop (dt1:DTree) := 
+forall f p ch dt2,
+  WF_dtree f dt1 ->
+  p `in` dtree_dom dt1 ->
+  imm_domination f p ch ->
+  dtree_insert dt1 p ch = dt2 ->
+  WF_dtree f dt2 /\ is_dtree_edge dt2 p ch /\
+  (is_dtree_edge dt1 p ch -> dt1 = dt2).
+
+Definition dtrees_insert__wf_dtrees_prop (dts1:DTrees) := 
+forall f p ch dts2 root,
+  WF_dtrees f root dts1 ->
+  p `in` dtrees_dom dts1 ->
+  imm_domination f p ch ->
+  dtrees_insert dts1 p ch = dts2 ->
+  WF_dtrees f root dts2 /\ is_dtrees_edge dts2 p ch /\
+  (is_dtrees_edge dts1 p ch -> dts1 = dts2).
+
+Lemma dtree_insert__wf_dtree_mutrec :
+  (forall dt1, dtree_insert__wf_dtree_prop dt1) *
+  (forall dts1, dtrees_insert__wf_dtrees_prop dts1).
+Proof.
+  apply dtree_mutrec; 
+    unfold dtree_insert__wf_dtree_prop, dtrees_insert__wf_dtrees_prop;
+    simpl; intros.
+Admitted.
+
+Lemma dtree_insert__wf_dtree : forall f p ch dt1 dt2,
+  WF_dtree f dt1 ->
+  p `in` dtree_dom dt1 ->
+  imm_domination f p ch ->
+  dtree_insert dt1 p ch = dt2 ->
+  WF_dtree f dt2 /\ is_dtree_edge dt2 p ch /\
+  (is_dtree_edge dt1 p ch -> dt1 = dt2).
+Admitted.
+
+Fixpoint create_dtree_from_chain dt chain : DTree :=
+match chain with
+| p::((ch::_) as chain') => 
+    create_dtree_from_chain (dtree_insert dt p ch) chain'
+| _ => dt
+end.
+
+Fixpoint chain_in_dtree chain dt : Prop :=
+match chain with
+| p::((ch::_) as chain') => 
+   is_dtree_edge dt p ch /\ chain_in_dtree chain' dt
+| _ => True
+end.
+
+Lemma create_dtree_from_chain__wf_dtree: forall f dt chain,
+  wf_chain f dt chain ->
+  WF_dtree f dt ->
+  WF_dtree f (create_dtree_from_chain dt chain).
+Admitted.
+
+Lemma create_dtree_from_chain__in_dtree: forall f dt chain,
+  wf_chain f dt chain ->
+  chain_in_dtree chain (create_dtree_from_chain dt chain).
+Admitted.
+
+Lemma create_dtree_from_chain__in_dtree': forall dt chain chain0,
+  chain_in_dtree chain0 dt ->
+  chain_in_dtree chain0 (create_dtree_from_chain dt chain).
+Admitted.
+
+Lemma create_dtree_from_chain__wf_chain: forall f chain0 chain dt,
+  wf_chain f dt chain0 ->
+  wf_chain f (create_dtree_from_chain dt chain) chain0.
+Proof.
+  induction chain; simpl; intros; auto.
+    destruct chain; auto.
+    apply IHchain.    
+
+Admitted.
+
+Definition create_dtree (f: fdef) : option DTree :=
+match getEntryLabel f, reachablity_analysis f with
+| Some root, Some rd =>
+    let dt := dom_analyze f in
+    let b := bound_fdef f in
+    let chains := compute_sdom_chains (dep_doms__nondep_doms b dt) rd in
+    Some (fold_left 
+      (fun acc elt => let '(_, chain):=elt in create_dtree_from_chain acc chain) 
+      chains (DT_node root DT_nil))
+| _, _ => None
+end.
+
+Lemma fold_left_create_dtree_from_chain__wf_dtree: forall f chains dt,
+  (forall l0 chain0, In (l0, chain0) chains -> wf_chain f dt chain0) ->
+  WF_dtree f dt ->
+  WF_dtree f
+    (fold_left
+       (fun (acc : DTree) (elt : l * list id) =>
+        let '(_, chain) := elt in create_dtree_from_chain acc chain) chains 
+       dt).
+Proof.
+  induction chains; simpl; intros; auto.
+    destruct a.
+    apply create_dtree_from_chain__wf_dtree with (chain:=l1) in H0; eauto.
+      apply IHchains; auto.
+        intros.
+        apply create_dtree_from_chain__wf_chain; eauto.
+Qed.
+
+Lemma fold_left_create_dtree_from_chain_init_in_dtree: forall chain0 chains dt,
+  chain_in_dtree chain0 dt ->
+  chain_in_dtree chain0
+    (fold_left
+      (fun (acc : DTree) (elt : l * list id) =>
+       let '(_, chain) := elt in create_dtree_from_chain acc chain)
+     chains dt).
+Proof.
+  induction chains; intros; auto.
+    apply IHchains. destruct a.
+    apply create_dtree_from_chain__in_dtree'; auto.
+Qed.
+
+Lemma fold_left_create_dtree_from_chain__in_dtree: forall f l0 chain0 chains dt,
+  In (l0, chain0) chains -> wf_chain f dt chain0 ->
+  chain_in_dtree chain0
+    (fold_left
+      (fun (acc : DTree) (elt : l * list id) =>
+       let '(_, chain) := elt in create_dtree_from_chain acc chain)
+     chains dt).
+Proof.
+  induction chains; simpl; intros.
+    inv H.
+
+    destruct H as [H | H]; subst.
+      apply fold_left_create_dtree_from_chain_init_in_dtree.
+      eapply create_dtree_from_chain__in_dtree; eauto.
+
+      apply IHchains; auto.
+      destruct a.
+      apply create_dtree_from_chain__wf_chain; eauto.
+Qed.
+
+Lemma create_dtree__wf_dtree: forall f dt,
+  create_dtree f = Some dt ->
+  WF_dtree f dt /\ 
+  match getEntryLabel f, reachablity_analysis f with
+  | Some root, Some rd =>
+      let dt' := dom_analyze f in
+      let b := bound_fdef f in
+      let chains := compute_sdom_chains (dep_doms__nondep_doms b dt') rd in
+      forall l0 chain0, 
+        In (l0, chain0) chains -> chain_in_dtree chain0 dt
+  | _, _ => True
+  end.
+Proof.
+  unfold create_dtree.
+  intros.
+  remember (getEntryLabel f) as R.
+  destruct R; tinv H.
+  remember (reachablity_analysis f) as R.
+  destruct R; inv H.
+  split. 
+    apply fold_left_create_dtree_from_chain__wf_dtree.
+      intros. eapply compute_sdom_chains__wf_chain; eauto.
+      apply WDT_node; auto.
+        admit. (*reach*)
+        constructor.
+    intros.
+    eapply fold_left_create_dtree_from_chain__in_dtree; eauto.
+      eapply compute_sdom_chains__wf_chain; eauto.    
+Qed.
+
 Fixpoint find_idom_aux (res: AMap.t (set l)) (acc:l) (dts: set l): option l :=
 match dts with
 | nil => Some acc
@@ -189,29 +535,94 @@ match AMap.get l0 res with
 | _ => None
 end.
 
-Require Import Trees.
-
-Fixpoint dtree_insert dt parent child : option DTree :=
-match dt with
-| DT_node l0 dts0 => 
-    if (id_dec parent l0) then 
-      Some (DT_node l0 (DT_cons (DT_node child DT_nil) dts0))
-    else 
-      match dtrees_insert dts0 parent child with
-      | Some dts1 => Some (DT_node l0 dts1)
-      | None => None
-      end
-end
-with dtrees_insert (dts: DTrees) parent child : option DTrees :=
-match dts with
-| DT_nil => Some DT_nil
-| DT_cons dt0 dts0 => 
-    match dtree_insert dt0 parent child, dtrees_insert dts0 parent child with
-    | Some dt1, Some dts1 => Some (DT_cons dt1 dts1)
-    | _, _ => None
+Fixpoint compute_idoms (res: AMap.t (set l)) (bd: list l) (acc: list (l * l)) :
+  list (l * l) :=
+match bd with
+| nil => acc
+| l0 :: bd' =>
+    match find_idom res l0 with
+    | None => compute_idoms res bd' acc
+    | Some l1 => compute_idoms res bd' ((l1,l0)::acc)
     end
 end.
 
+(*
+Require Import Orders.
+
+Module NatOrder <: TotalLeBool.
+
+Section A.
+ 
+  Variable f: fdef.
+  Variable l0: l.
+  Hypothesis Hreach: reachable f l0.
+
+  Definition t := {l0: l & }.
+  Fixpoint leb x y :=
+    match x, y with
+    | O, _ => true
+    | _, O => false
+    | S x', S y' => leb x' y'
+    end.
+  Infix "<=?" := leb (at level 35).
+  Theorem leb_total : forall a1 a2, a1 <=? a2 \/ a2 <=? a1. admit. Qed.
+
+End A.
+
+End NatOrder.
+
+Lemma sdom_ordered : forall f l1 l2 l3
+  (Hneq: l1 <> l2) (Hreach: reachable f l3)
+  (Hsdom: strict_domination f l1 l3)
+  (Hsdom': strict_domination f l2 l3),
+  strict_domination f l1 l2 \/ strict_domination f l2 l1.
+Proof.
+  intros.
+  apply sdom_sdom' in Hsdom; auto.
+  apply sdom_sdom' in Hsdom'; auto.
+  assert (J:=Hsdom').
+  eapply sdom_ordered' in J; eauto.
+  destruct J as [[J1 J2] | [J1 J2]].
+    left. apply dom_sdom; auto.
+    right. apply dom_sdom; auto.
+Qed.
+
+Require Import Sorting.
+
+Module Import NatSort := Sort NatOrder.
+
+Check sort.
+
+Eval compute in sort (5::3::6::1::8::6::0::nil)%nat.
+*)
+
+(*
+Fixpoint find_idom_aux (res: AMap.t (set l)) (acc:l) (dts: set l): option l :=
+match dts with
+| nil => Some acc
+| l0::dts' =>
+    match AMap.get l0 res, AMap.get acc res with
+    | dts1, dts2 =>
+        if (in_dec l_dec l0 dts2)
+        then (* acc << l0 *)
+          find_idom_aux res acc dts' 
+        else
+          if (in_dec l_dec acc dts1)
+          then (* l0 << acc *)
+            find_idom_aux res l0 dts' 
+          else (* l0 and acc are incompariable *)
+            None
+    end
+end.
+
+(* We should prove that this function is not partial. *)
+Definition find_idom (res: AMap.t (set l)) (l0:l) : option l :=
+match AMap.get l0 res with
+| l1::dts0 => find_idom_aux res l1 dts0
+| _ => None
+end.
+
+(*
 Fixpoint tree2dtree vs es (tree: Tree vs es) : option DTree :=
 match tree with
 | T_root (index le) => Some (DT_node le DT_nil)
@@ -222,8 +633,9 @@ match tree with
     end
 | T_eq vs1 vs2 es1 es2 _ _ t1 => tree2dtree vs1 es1 t1
 end.
+*)
 
-Definition PreDTree := list (l * l).
+Definition PreDTree := list (l * list l).
 
 Definition getEntryLabel (f:fdef) : option l :=
 match f with
@@ -234,206 +646,166 @@ end.
 Fixpoint cdom (pdt: PreDTree) : atoms :=
 match pdt with
 | nil => empty
-| (_,l2)::pdt' => add l2 (cdom pdt')
+| (_, children)::pdt' => 
+    fold_left (fun acc child => add child acc) children (cdom pdt') 
 end.
 
-Inductive WF_pre_dtree (f:fdef) : PreDTree -> Type :=
-| WPDT_entry : forall entry child,
+Inductive WF_idoms f : list (l*l) -> Prop :=
+| WF_idoms_nil : WF_idoms f nil 
+| WF_idoms_cons : forall l1 l2 idoms, 
+    imm_domination f l1 l2 -> WF_idoms f idoms ->
+    WF_idoms f ((l1,l2)::idoms)
+.
+
+Inductive WF_predtree (f:fdef) : PreDTree -> Prop :=
+| WPDT_entry : forall entry children,
     getEntryLabel f = Some entry ->
-    imm_domination f entry child -> 
-    WF_pre_dtree f ((entry, child)::nil)
-| WPDT_cons : forall parent child pdt,
-    WF_pre_dtree f pdt ->
+    (forall child, In child children -> imm_domination f entry child) ->
+    NoDup children ->
+    WF_predtree f ((entry, children)::nil)
+| WPDT_cons : forall parent children pdt,
+    WF_predtree f pdt ->
     reachable f parent ->
-    imm_domination f parent child -> 
-    child `notin` dom pdt `union` cdom pdt ->
-    (parent `in` dom pdt \/ exists ancestor, In (ancestor, parent) pdt) -> 
-    WF_pre_dtree f ((parent, child) :: pdt).
+    (forall child, In child children -> 
+       imm_domination f parent child /\ child `notin` dom pdt `union` cdom pdt) ->
+    NoDup children ->
+    parent `notin` dom pdt ->
+    (exists ancestor, exists parents,
+      In (ancestor, parents) pdt /\ In parent parents) -> 
+    WF_predtree f ((parent, children) :: pdt).
 
-Definition arcs_of_pre_dtree (pdt: PreDTree) : A_set :=
-fun arc =>
-  match arc with
-  | A_ends (index parent) (index child) => 
-      In (parent, child) pdt \/ In (child, parent) pdt
-  end.
+Fixpoint dtree_insert dt parent children : option DTree :=
+match dt with
+| DT_node l0 dts0 => 
+    if (id_dec parent l0) then 
+      Some (DT_node l0 
+        (fold_left (fun acc child => DT_cons (DT_node child DT_nil) acc) 
+          children dts0))
+    else 
+      match dtrees_insert dts0 parent children with
+      | Some dts1 => Some (DT_node l0 dts1)
+      | None => None
+      end
+end
+with dtrees_insert (dts: DTrees) parent children : option DTrees :=
+match dts with
+| DT_nil => Some DT_nil
+| DT_cons dt0 dts0 => 
+    match dtree_insert dt0 parent children, 
+          dtrees_insert dts0 parent children with
+    | Some dt1, Some dts1 => Some (DT_cons dt1 dts1)
+    | _, _ => None
+    end
+end.
 
-Definition vertexes_of_pre_dtree (pdt: PreDTree) : V_set :=
-fun v =>
-  match v with
-  | index n => exists n', In (n, n') pdt \/ In (n', n) pdt
-  end.
+Fixpoint predtree2dtree (pdt: PreDTree) : option DTree :=
+match pdt with
+| nil => None
+| (p, chs) :: nil =>
+    Some (DT_node p
+      (fold_left (fun acc child => DT_cons (DT_node child DT_nil) acc) 
+         chs DT_nil))
+| (p, chs) :: pdt' =>
+    match predtree2dtree pdt' with
+    | Some dt' => dtree_insert dt' p chs
+    | _ => None
+    end
+end.
 
-Lemma In_vertexes_of_pre_dtree: forall l1 l2 pdt,
-  In (l1, l2) pdt -> vertexes_of_pre_dtree pdt (index l2).
+Lemma wf_predtree__wf_dtree__helper: forall f p chs dts0
+  (H0 : reachable f p)
+  (H1 : forall child : l, In child chs -> 
+        imm_domination f p child /\ child `notin` dtrees_dom dts0)
+  (h2 : NoDup chs),
+  WF_dtrees f p dts0 ->
+  WF_dtrees f p
+       (fold_left
+          (fun (acc : DTrees) (child : l) =>
+           DT_cons (DT_node child DT_nil) acc) chs dts0).
 Proof.
-  induction pdt; simpl; intros.
-    inv H.
-    exists l1.
-    destruct H as [H | H]; subst; auto.
-Qed.
+  induction chs; simpl; intros; auto.
+    inv h2.
+    apply IHchs; auto.
+      intros.
+      assert (a = child \/ In child chs) as Hin. auto.
+      apply H1 in Hin.
+      destruct Hin as [J1 J2].
+      simpl. split; auto.
+      assert (child <> a) as Hneq.
+        destruct (l_dec child a); subst; auto.
+          fsetdec.
 
-Lemma In_vertexes_of_pre_dtree': forall l1 l2 pdt,
-  In (l1, l2) pdt -> vertexes_of_pre_dtree pdt (index l1).
-Proof.
-  induction pdt; simpl; intros.
-    inv H.
-    exists l2.
-    destruct H as [H | H]; subst; auto.
-Qed.
-
-Lemma InDom_vertexes_of_pre_dtree: forall l1 pdt,
-  l1 `in` dom pdt -> vertexes_of_pre_dtree pdt (index l1).
-Proof.
-  induction pdt; simpl; intros.
-    fsetdec.
-
-    destruct a.
-    assert (l1 = a \/ l1 `in` dom pdt) as Hin.
-      fsetdec.
-    destruct Hin as [Hin | Hin]; subst.
-      exists l0. auto.
-      apply IHpdt in Hin. simpl in Hin.
-      destruct Hin as [n' [Hin | Hin]]; exists n'; auto.
-Qed.
-
-Lemma Notin_vertexes_of_pre_dtree: forall child pdt
-  (n : child `notin` dom pdt `union` cdom pdt),
-  ~ vertexes_of_pre_dtree pdt (index child).
-Proof.
-  induction pdt; simpl; intros.
-    intro J. destruct J as [_ [J | J]]; inv J.
-
-    intro J. 
-    destruct J as [n' [J | J]].
-      destruct J as [J | J]; subst.
+      assert (a = a \/ In a chs) as Hin. auto.
+      apply H1 in Hin.
+      destruct Hin as [J1 J2].
+      apply WDT_cons; simpl; auto.
         fsetdec.
-        
-        destruct a.    
-        apply In_vertexes_of_pre_dtree' in J.
-        revert J. 
-        apply IHpdt; auto.
-      destruct J as [J | J]; subst.
-        fsetdec.
-
-        destruct a.    
-        apply In_vertexes_of_pre_dtree in J.
-        revert J. 
-        apply IHpdt; auto.
+        apply WDT_node; auto.
+          admit.
+          apply WDT_nil.
 Qed.
 
-Lemma In_arcs_of_pre_dtree: forall a a0 pdt,
-  In (a, a0) pdt ->
-  Ensembles.In Arc (arcs_of_pre_dtree pdt) (A_ends (index a) (index a0)).
-Proof.
-  induction pdt; simpl; intros.
-    inv H.
+Scheme dtree_rec2 := Induction for DTree Sort Set
+  with dtrees_rec2 := Induction for DTrees Sort Set.
 
-    unfold Ensembles.In. simpl.
-    destruct H as [H | H]; subst; auto.
+Definition dtree_mutrec P P' :=
+  fun h1 h2 h3 => 
+    (pair (@dtree_rec2 P P' h1 h2 h3) (@dtrees_rec2 P P' h1 h2 h3)).
+
+Definition dtree_insert__wf_dtree_prop (dt1:DTree) := 
+forall f a1 a0,
+  WF_dtree f dt1 ->
+  exists dt2, dtree_insert dt1 a1 a0 = ret dt2 /\ WF_dtree f dt2.
+
+Definition dtrees_insert__wf_dtrees_prop (dts1:DTrees) := 
+forall f root a1 a0,
+  WF_dtrees f root dts1 ->
+  exists dts2, dtrees_insert dts1 a1 a0 = ret dts2 /\ WF_dtrees f root dts2.
+
+Lemma dtree_insert__wf_dtree_mutrec :
+  (forall dt1, dtree_insert__wf_dtree_prop dt1) *
+  (forall dts1, dtrees_insert__wf_dtrees_prop dts1).
+Proof.
+  apply dtree_mutrec; 
+    unfold dtree_insert__wf_dtree_prop, dtrees_insert__wf_dtrees_prop;
+    simpl; intros.
+Admitted.
+
+Lemma dtree_insert__wf_dtree: forall f dt1 a1 a0,
+  WF_dtree f dt1 ->
+  exists dt2, dtree_insert dt1 a1 a0 = ret dt2 /\ WF_dtree f dt2.
+Proof.
+  destruct dtree_insert__wf_dtree_mutrec as [J1 _].
+  unfold dtree_insert__wf_dtree_prop in J1. auto.
 Qed.
 
-Lemma In_arcs_of_pre_dtree': forall a a0 pdt,
-  In (a0, a) pdt ->
-  Ensembles.In Arc (arcs_of_pre_dtree pdt) (A_ends (index a) (index a0)).
+Lemma WF_idoms_elim: forall f p ch idoms,
+  WF_idoms f idoms -> In (p, ch) idoms -> imm_domination f p ch.
+Admitted.
+
+Lemma wf_predtree__wf_dtree : forall f pdts,
+  WF_predtree f pdts ->
+  exists dt, predtree2dtree pdts = Some dt /\ WF_dtree f dt.
 Proof.
-  induction pdt; simpl; intros.
-    inv H.
+  intros.
+  induction H; simpl.
+    exists 
+      (DT_node entry
+         (fold_left
+            (fun (acc : DTrees) (child : l) =>
+             DT_cons (DT_node child DT_nil) acc) children DT_nil)).
+    split; auto.
+      apply WDT_node.
+        admit.
+        admit.
+        apply wf_predtree__wf_dtree__helper; auto.
+          admit. 
+          apply WDT_nil.
 
-    unfold Ensembles.In. simpl.
-    destruct H as [H | H]; subst; auto.
-Qed.
-
-Lemma WF_pre_dtree_isa_tree: forall f pdt, 
-  WF_pre_dtree f pdt -> 
-  Tree (vertexes_of_pre_dtree pdt) (arcs_of_pre_dtree pdt).
-Proof.
-  intros f pdt Hwf.
-  induction Hwf.
-    apply T_eq with 
-      (v:=V_union (V_single (index child)) (V_single (index entry)))
-      (a:=A_union (E_set (index entry) (index child)) A_empty).
-      apply U_set_eq.
-        intros x.
-        split; intro J.
-          inv J; inv H; simpl.
-            exists entry. auto.
-            exists child. auto.
-          destruct x; simpl in J.
-          destruct J as [n' [J | J]].
-            destruct J as [J | J]; inv J. 
-            apply In_right. apply In_single; auto.
-
-            destruct J as [J | J]; inv J. 
-            apply In_left. apply In_single; auto.
-      apply A_set_eq.
-        intros x.
-        split; intro J.
-          inv J; inv H; simpl; auto.
-
-          destruct x as [[] []]; simpl in J.
-          destruct J as [J | J].
-            destruct J as [J | J]; inv J. 
-            apply In_left. apply E_right.
-
-            destruct J as [J | J]; inv J. 
-            apply In_left. apply E_left.
-      apply T_leaf.
-        apply T_root.
-        apply In_single; auto.
-
-        intro J. inv J. 
-        unfold imm_domination, strict_domination in i0.
-        destruct i0 as [[_ J] _]; auto.
-
-    apply T_eq with 
-      (v:=V_union (V_single (index child)) (vertexes_of_pre_dtree pdt))
-      (a:=A_union (E_set (index parent) (index child)) (arcs_of_pre_dtree pdt)).
-      apply U_set_eq.
-        intros [v].
-        split; intro J.
-          inv J; inv H.
-            exists parent. simpl. auto.
-
-            destruct H0 as [H0 | H0].
-              eapply In_vertexes_of_pre_dtree'; simpl; eauto.
-              eapply In_vertexes_of_pre_dtree; simpl; eauto.
-
-          destruct J as [n' [J | J]]; simpl in J.
-            apply In_right. 
-            destruct J as [J | J].
-              inv J. 
-              clear - o. destruct o as [o | [anc e]].
-                eapply InDom_vertexes_of_pre_dtree; eauto.
-                apply In_vertexes_of_pre_dtree in e; auto.
-
-              apply In_vertexes_of_pre_dtree' in J; auto.
-            destruct J as [J | J].
-              inv J. 
-              apply In_left. apply In_single.
-
-              apply In_right. 
-              apply In_vertexes_of_pre_dtree in J; auto.
-      apply A_set_eq.
-        intros [v1 v2]. destruct v1, v2.
-        split; intro J.
-          inv J; inv H; simpl; auto.
-
-          inv J.
-            simpl in H. 
-            destruct H as [H | H].
-              inv H.
-              apply In_left. apply E_right.
-              apply In_right. apply In_arcs_of_pre_dtree; auto.
-            simpl in H. 
-            destruct H as [H | H].
-              inv H.
-              apply In_left. apply E_left.
-              apply In_right. apply In_arcs_of_pre_dtree'; auto.
-      apply T_leaf; auto.
-        clear - o. destruct o as [o | [anc e]].
-          eapply InDom_vertexes_of_pre_dtree; eauto.
-          apply In_vertexes_of_pre_dtree in e; auto.
-        apply Notin_vertexes_of_pre_dtree; auto.
+    destruct pdt; tinv H.
+    destruct IHWF_predtree as [dt [J1 J2]].
+    rewrite J1.
+    apply dtree_insert__wf_dtree; auto.
 Qed.
 
 Fixpoint find_children (res: AMap.t (set l)) (root:l) 
@@ -536,9 +908,7 @@ Proof.
         intros x Jx. 
         apply H1.
         apply remove_neq_in' in Jx; auto.
-        destruct (id_dec x a); subst; auto.
-        contradict Jx. apply remove_In.
-
+        destruct Jx as [Jx1 Jx2]; auto.
         omega.
 
         intro J0. inv J0.
@@ -557,110 +927,497 @@ Proof.
     apply incl_refl.
 Qed.
 
-Fixpoint compute_idoms (res: AMap.t (set l)) (bd: list l) (acc: list (l * l)) :
-  list (l * l) :=
-match bd with
-| nil => acc
-| l0 :: bd' =>
-    match find_idom res l0 with
-    | None => compute_idoms res bd' acc
-    | Some l1 => compute_idoms res bd' ((l1,l0)::acc)
+Fixpoint find_next_children (idoms: list (l * l)) (parent: l) (acc : list l)
+  (others: set l) : list l * set l :=
+match idoms with
+| nil => (acc, others)
+| (l1, l2)::idoms' =>
+    if (l_dec l1 parent) then 
+      if (in_dec l_dec l2 others) then
+        find_next_children idoms' parent (l2::acc) (List.remove l_dec l2 others)
+      else find_next_children idoms' parent acc others
+    else find_next_children idoms' parent acc others
+end.
+
+Fixpoint find_next_children_from_children (idoms: list (l * l)) (children:list l)
+  (others: set l) : option (l * list l * set l) :=
+match children with
+| nil => None
+| ch::children' =>
+    match find_next_children idoms ch nil others with
+    | (nil, _) => find_next_children_from_children idoms children' others
+    | (children0, others') => Some (ch, children0, others')
     end
 end.
 
-Fixpoint find_next_child (idoms: list (l * l)) (parent: l) (others:set l) 
-  : option l :=
-match idoms with
-| nil => None
-| (l1, l2)::idoms' =>
-    if (l_dec l1 parent) then 
-      if (in_dec l_dec l2 others) then Some l2
-      else find_next_child idoms' parent others
-    else find_next_child idoms' parent others
-end.
-
-Fixpoint find_next_sub_pre_dtree_aux (idoms: list (l * l)) (pdt0 pdt:PreDTree) 
+Fixpoint find_next_sub_predtree_aux (idoms: list (l * l)) (pdt0 pdt:PreDTree) 
   (others:set l) : option (PreDTree * set l) :=
 match pdt with
 | nil => None
-| (p, ch)::pdt' => 
-    match find_next_child idoms ch others with
-    | None => 
-        match find_next_child idoms p others with
-        | None => 
-            find_next_sub_pre_dtree_aux idoms pdt0 pdt' others
-        | Some ch' =>
-            Some ((p, ch')::pdt0, List.remove l_dec ch' others)
-        end
-    | Some ch' => Some ((ch, ch')::pdt0, List.remove l_dec ch' others)
+| (p, chs)::pdt' => 
+    match find_next_children_from_children idoms chs others with
+    | None => find_next_sub_predtree_aux idoms pdt0 pdt' others
+    | Some (ch, chs', others') => Some ((ch, chs')::pdt0, others')
     end
 end.
 
-Definition find_next_sub_pre_dtree (idoms: list (l * l)) (pdt:PreDTree) 
+Definition find_next_sub_predtree (idoms: list (l * l)) (pdt:PreDTree) 
   (others:set l) : option (PreDTree * set l) :=
-find_next_sub_pre_dtree_aux idoms pdt pdt others.
+find_next_sub_predtree_aux idoms pdt pdt others.
 
-Lemma find_next_child_inv : forall idoms l1 others l2,
-  find_next_child idoms l1 others = ret l2 ->
-  In l2 others /\ In (l1, l2) idoms.
+Lemma in_singleton_inv: forall A (a b:A), In a [b] -> a = b.
+Proof.
+  intros.
+  simpl in H. destruct H; auto. inv H.
+Qed.
+
+Lemma find_next_children_inv : forall p idoms chs others chs' others',
+  find_next_children idoms p chs others = (chs', others') ->
+  exists chs'', chs' = chs'' ++ chs /\
+    others' = fold_right (fun ch acc => List.remove l_dec ch acc) others chs'' /\
+    (forall ch, In ch chs'' -> In ch others /\ In (p, ch) idoms).
 Proof.
   induction idoms; simpl; intros.
     inv H.
+    exists nil. simpl.
+    split; auto.
+    split; auto. 
+      intros. inversion H.
 
     destruct a.
-    destruct (l_dec l0 l1); subst.
-      destruct (in_dec l_dec l3 others).
-        inv H. auto.
-        apply IHidoms in H. destruct H. split; auto.
-      apply IHidoms in H. destruct H. split; auto.
+    destruct (l_dec l0 p); subst.
+      destruct (in_dec l_dec l1 others).
+        apply IHidoms in H.
+        destruct H as [chs'' [J1 [J2 J3]]]; subst.
+        exists (chs''++[l1]).
+        simpl_env.
+        split; auto.
+        split.
+          rewrite fold_right_app. simpl. auto.
+
+          intros ch Hin.
+          apply in_app_or in Hin.
+          destruct Hin as [Hin | Hin].
+            apply J3 in Hin.
+            destruct Hin as [J2 J4].
+            split; auto.
+              apply remove_neq_in' in J2.
+              destruct J2; auto.
+
+            apply in_singleton_inv in Hin; subst.
+            split; auto.
+    
+        apply IHidoms in H.
+        destruct H as [chs'' [J1 [J2 J3]]]; subst.
+        exists chs''.
+        split; auto.
+        split; auto.
+          intros ch Hin.
+          apply J3 in Hin.
+          destruct Hin as [J2 J4].
+          split; auto.
+      apply IHidoms in H.
+      destruct H as [chs'' [J1 [J2 J3]]]; subst.
+      exists chs''.
+      split; auto.
+      split; auto.
+        intros ch Hin.
+        apply J3 in Hin.
+        destruct Hin as [J2 J4].
+        split; auto.
 Qed.       
 
-Lemma find_next_sub_pre_dtree_aux_length: forall idoms pdt0 acc others acc' others',
-  find_next_sub_pre_dtree_aux idoms pdt0 acc others = ret (acc', others') ->
+Lemma find_next_children_from_children_inv: forall idoms chs others ch chs' others',
+  find_next_children_from_children idoms chs others = ret (ch, chs', others') ->
+  others' = fold_right (fun ch0 acc => List.remove l_dec ch0 acc) others chs' /\
+  In ch chs /\ (forall ch', In ch' chs' -> In ch' others /\ In (ch, ch') idoms)
+  /\ chs' <> nil.
+Proof.
+  induction chs; simpl; intros.
+    inv H.
+
+    remember (find_next_children idoms a nil others) as R.
+    destruct R.
+    destruct l0; auto.
+      apply IHchs in H.
+      destruct H as [J1 [J2 J3]].
+      split; auto.
+
+      inv H.
+      symmetry in HeqR.
+      apply find_next_children_inv in HeqR; auto.
+      destruct HeqR as [chs'' [J1 [J2 J3]]]; subst.
+      simpl_env in J1. subst.
+      split; auto.
+      split; auto.
+      split; auto.
+        intro J. inv J.
+Qed.
+
+Lemma find_next_sub_predtree_aux_inv: forall idoms pdt0 pdt others pdt' 
+  others',
+  find_next_sub_predtree_aux idoms pdt0 pdt others = Some (pdt', others') ->
+  exists p, exists chs, 
+    pdt' = (p,chs)::pdt0 /\ 
+    others' = fold_right (fun ch0 acc => List.remove l_dec ch0 acc) others chs /\
+    (forall ch, In ch chs -> In ch others /\ In (p, ch) idoms) /\ chs <> nil /\
+    exists p', exists chs', In (p', chs') pdt /\ In p chs'.
+Proof.
+  induction pdt; simpl; intros.
+    inv H.
+
+    destruct a.
+    remember (find_next_children_from_children idoms l1 others) as R.
+    destruct R as [[[ch ch'] others'']|].
+      inv H.
+      exists ch. exists ch'. 
+      symmetry in HeqR.
+      apply find_next_children_from_children_inv in HeqR.
+      destruct HeqR as [J1 [J2 [J3 J4]]]; subst.
+      split; auto.
+      split; auto.
+      split; auto.
+      split; auto.
+        exists l0. exists l1. split; auto.
+
+      apply IHpdt in H; auto.
+      destruct H as [p [chs [Heq1 [Heq2 [J1 [J0 [p' [chs' [J2 J3]]]]]]]]]; 
+        subst.
+      exists p. exists chs. 
+      split; auto.
+      split; auto.
+      split; auto.
+      split; auto.
+        exists p'. exists chs'. split; auto.
+Qed.
+
+Lemma find_next_sub_predtree_inv: forall idoms pdt others pdt' 
+  others',
+  find_next_sub_predtree idoms pdt others = Some (pdt', others') ->
+  exists p, exists chs, 
+    pdt' = (p,chs)::pdt /\ 
+    others' = fold_right (fun ch0 acc => List.remove l_dec ch0 acc) others chs /\
+    (forall ch, In ch chs -> In ch others /\ In (p, ch) idoms) /\ chs <> nil /\
+    exists p', exists chs', In (p', chs') pdt /\ In p chs'.
+Proof.
+  intros. unfold find_next_sub_predtree in H.
+  apply find_next_sub_predtree_aux_inv in H; auto.
+Qed.
+
+Lemma fold_right_remove_length: forall chs others
+  (J1 : forall ch : l, In ch chs -> In ch others)
+  (J0 : chs <> nil),
+  (length
+     (fold_right
+        (fun (ch0 : l) (acc0 : list l) => List.remove l_dec ch0 acc0) others
+        chs) < length others)%nat.
+Proof.
+  induction chs; simpl; intros.
+    congruence.
+
+    destruct chs.
+      simpl.
+      apply remove_in_length; auto.
+
+      assert (length
+               (fold_right
+                  (fun (ch0 : l) (acc0 : list l) => List.remove l_dec ch0 acc0)
+                  others (l0::chs)) < length others)%nat as J.
+        apply IHchs; auto.
+          intro J. inv J.
+      assert (G:=@remove_length _ l_dec a (fold_right
+                  (fun (ch0 : l) (acc0 : list l) => List.remove l_dec ch0 acc0)
+                  others (l0::chs))).
+      omega.
+Qed.
+
+Lemma find_next_sub_predtree_length: forall idoms acc others acc' others',
+  find_next_sub_predtree idoms acc others = ret (acc', others') ->
   (length others' < length others)%nat.
 Proof.
+  intros.
+  apply find_next_sub_predtree_inv in H.
+  destruct H as [p [chs [Heq1 [Heq2 [J1 [J0 [p' [chs' [J2 J3]]]]]]]]]; subst.
+  apply fold_right_remove_length; auto.
+  intros ch Hin. apply J1 in Hin. destruct Hin; auto.
+Qed.
+
+Program Fixpoint create_predtree_aux (others:set l) (idoms: list (l * l)) 
+  (acc:PreDTree) {measure (List.length others)} : option PreDTree :=
+match others with
+| nil => Some acc
+| _ =>
+   match find_next_sub_predtree idoms acc others with
+   | None => None
+   | Some (acc', others') => create_predtree_aux others' idoms acc'
+   end
+end.
+Next Obligation. 
+  eapply find_next_sub_predtree_length; eauto.
+Qed.
+
+Fixpoint init_predtree (idoms: list (l * l)) (root:l) (others:set l)
+  : option (PreDTree * list l) :=
+match find_next_children idoms root nil others with
+| (nil, _) => None
+| (children, others') => Some ([(root, children)], others')
+end.
+
+Definition create_dtree (f: fdef) : option DTree :=
+match getEntryBlock f, reachablity_analysis f with
+| Some (block_intro root _ _ _), Some rd =>
+    let dt := dom_analyze f in
+    let b := bound_fdef f in
+    let idoms := compute_idoms (dep_doms__nondep_doms b dt) rd nil in
+    match init_predtree idoms root (List.remove eq_atom_dec root rd) with
+    | None => None
+    | Some (pdt0, others) =>
+        match (create_predtree_aux others idoms pdt0) with
+        | None => None
+        | Some pdt => predtree2dtree pdt
+        end
+    end
+| _, _ => None
+end.
+
+Lemma in_predtree_dom: forall p chs (pdt0:PreDTree),
+  In (p, chs) pdt0 -> p `in` dom pdt0.
+Proof.
+  induction pdt0; simpl; intros.
+    inv H.
+    destruct H as [H | H]; subst.
+      fsetdec.
+
+      destruct a.
+      apply IHpdt0 in H.
+      fsetdec.
+Qed.
+
+Lemma in_fold_left_atoms: forall ch chs init
+  (H0 : In ch chs \/ ch `in` init),
+  ch `in` fold_left (fun (acc : atoms) (child : atom) => add child acc) chs init.
+Proof.
+  induction chs; simpl; intros.
+    destruct H0; auto.
+      inv H.
+    destruct H0 as [[H0 | H0] | H0]; subst; eauto.
+Qed.
+
+Lemma in_predtree_cdom: forall p chs ch pdt0,
+  In (p, chs) pdt0 -> In ch chs -> ch `in` cdom pdt0.
+Proof.
+  induction pdt0; simpl; intros.
+    inv H.
+    destruct H as [H | H]; subst.
+      apply in_fold_left_atoms; auto.
+    destruct a.
+    apply in_fold_left_atoms; auto.
+Qed.
+
+Definition P_create_predtree_aux__WF_predtree (n:nat) :=
+  forall f idoms (Hwfi: WF_idoms f idoms) pdt0 others pdt
+  (Hdis: forall l0, 
+    In l0 others -> 
+    l0 `notin` dom pdt0 `union` cdom pdt0),
+  List.length others = n ->
+  WF_predtree f pdt0 ->
+  create_predtree_aux others idoms pdt0 = Some pdt ->
+  WF_predtree f pdt.
+
+Require Import Program.
+
+Ltac simple_create_predtree_aux :=
+  unfold create_predtree_aux, create_predtree_aux_func;
+  rewrite WfExtensionality.fix_sub_eq_ext;
+  repeat fold_sub create_predtree_aux_func ; simpl proj1_sig;
+  simpl. 
+
+Lemma in_fold_right_remove: forall p chs others
+  (Hin : In p
+          (fold_right
+             (fun (ch0 : l) (acc : list l) => List.remove l_dec ch0 acc)
+             others chs)),
+  In p others /\ ~ In p chs.
+Proof.
+  induction chs; simpl; intros.
+    split; auto.
+
+    apply remove_neq_in' in Hin; auto.
+    destruct Hin as [J1 J2].
+    apply IHchs in J1.
+    destruct J1 as [J1 J3].
+    split; auto.
+      intro J. destruct J as [J | J]; auto.
+Qed.
+
+Lemma notin_fold_left_atoms: forall ch chs init,
+  ~ In ch chs -> ch `notin` init -> 
+  ch `notin` 
+    fold_left (fun (acc : atoms) (child : atom) => add child acc) chs init.
+Proof.
+  induction chs; simpl; intros; auto.
+Qed.
+
+Lemma find_next_sub_predtree_fresh: forall (pdt0 : list (atom * list l)) idoms
+  (others : list atom) (pdt : PreDTree)
+  (Hdis : forall l0 : atom,
+          In l0 others -> l0 `notin` union (dom pdt0) (cdom pdt0))
+  (acc' : PreDTree) (others' : set l)
+  (HeqR : ret (acc', others') =
+          find_next_sub_predtree idoms pdt0 others),
+  forall l0 : atom, In l0 others' -> l0 `notin` union (dom acc') (cdom acc').
+Proof.
+  intros.
+  symmetry in HeqR.
+  apply find_next_sub_predtree_inv in HeqR.
+  destruct HeqR as [p [chs [Heq [J1 [J2 [J3 [p' [chs' [J4 J5]]]]]]]]]; subst.
+  simpl.
+  apply in_fold_right_remove in H.
+  destruct H as [J6 J7].
+  apply Hdis in J6.
+  assert (l0 `notin` 
+       (fold_left (fun (acc : atoms) (child : atom) => add child acc)
+          chs (cdom pdt0))) as J8.
+    apply notin_fold_left_atoms; auto.
+  assert (l0 <> p) as Hneq.
+    destruct (l_dec l0 p); subst; auto.
+    eapply in_predtree_cdom in J4; eauto.
+  fsetdec.
+Qed.
+
+Lemma WF_predtree__reachable: forall f pdt p chs ch,
+  WF_predtree f pdt ->
+  In (p, chs) pdt ->
+  In ch chs ->
+  reachable f ch.
+Admitted.
+
+Lemma find_next_sub_predtree_wf_predtree: 
+  forall f idoms (Hwfi: WF_idoms f idoms) pdt (Hwf:WF_predtree f pdt) 
+    others pdt' others'
+  (Hdis: forall l0, 
+    In l0 others -> 
+    l0 `notin` dom pdt `union` cdom pdt),
+  find_next_sub_predtree idoms pdt others = ret (pdt', others') ->
+  WF_predtree f pdt'.
+Proof.
+  intros.
+  apply find_next_sub_predtree_inv in H.
+  destruct H as [p [chs [Heq [J1 [J2 [J3 [p' [chs' [J4 J5]]]]]]]]]; subst.
+  apply WPDT_cons; auto.
+    eapply WF_predtree__reachable in J4; eauto.
+
+    intros child Hin.
+    apply J2 in Hin.
+    destruct Hin as [Hin1 Hin2].
+    split; auto.
+      eapply WF_idoms_elim; eauto.
+
+    admit.
+
+    
+
+Lemma find_next_sub_predtree_aux_wf_predtree: 
+  forall f idoms (Hwfi: WF_idoms f idoms) acc prefix 
+    (Hwf:WF_predtree f (prefix++acc)) others acc' others'
+  (Hdis: forall l0, 
+    In l0 others -> 
+    l0 `notin` dom (prefix++acc) `union` cdom (prefix++acc)),
+  find_next_sub_predtree_aux idoms (prefix++acc) acc others = 
+    ret (acc', others') ->
+  WF_predtree f acc'.
+Proof.
+  intros.
+  applu 
+
+
   induction acc; simpl; intros.
-    inv H. 
+    congruence.
 
     destruct a.
     remember (find_next_child idoms l1 others) as R.
     destruct R.
       inv H.
-      symmetry in HeqR.
-      apply find_next_child_inv in HeqR.
-      destruct HeqR.
-      apply remove_in_length; auto.
+      apply WPDT_cons; auto.
+        apply WF_predtree__reachable with (l1:=l0)(l2:=l1) in Hwf.
+          destruct Hwf; auto.
+          apply in_middle.
+        eapply find_next_child__imm_domination; eauto.
+
+        symmetry in HeqR.
+        apply find_next_child_inv in HeqR.
+        destruct HeqR as [J1 J2]. auto.
+
+        right.
+        exists l0. apply in_middle.
 
       remember (find_next_child idoms l0 others) as R.
-      destruct R; eauto.
+      destruct R.
         inv H.
-        symmetry in HeqR0.
-        apply find_next_child_inv in HeqR0.
-        destruct HeqR0.
-        apply remove_in_length; auto.
+        apply WPDT_cons; auto.
+          apply WF_predtree__reachable with (l1:=l0)(l2:=l1) in Hwf.
+            destruct Hwf; auto.
+            apply in_middle.
+          eapply find_next_child__imm_domination; eauto.
+
+          symmetry in HeqR0.
+          apply find_next_child_inv in HeqR0.
+          destruct HeqR0 as [J1 J2]. auto.
+          left. simpl_env. fsetdec.
+      rewrite_env ((prefix ++ [(l0, l1)]) ++ acc) in H.
+      apply IHacc in H; simpl_env; simpl; auto.
 Qed.
 
-Lemma find_next_sub_pre_dtree_length: forall idoms acc others acc' others',
-  find_next_sub_pre_dtree idoms acc others = ret (acc', others') ->
-  (length others' < length others)%nat.
+Lemma find_next_sub_predtree_wf_predtree: 
+  forall f idoms (Hwfi: WF_idoms f idoms) pdt (Hwf:WF_predtree f pdt) 
+    others pdt' others'
+  (Hdis: forall l0, 
+    In l0 others -> 
+    l0 `notin` dom pdt `union` cdom pdt),
+  find_next_sub_predtree idoms pdt others = ret (pdt', others') ->
+  WF_predtree f pdt'.
 Proof.
   intros.
-  unfold find_next_sub_pre_dtree in H.
-  apply find_next_sub_pre_dtree_aux_length in H; auto.
+  unfold find_next_sub_predtree in H.
+  change pdt with (nil++pdt) in H, Hdis at 1.
+  eapply find_next_sub_predtree_aux_wf_predtree in H; eauto.
 Qed.
 
-Program Fixpoint create_pre_dtree_aux (others:set l) (idoms: list (l * l)) 
-  (acc:PreDTree) {measure (List.length others)} : option PreDTree :=
-match others with
-| nil => Some acc
-| _ =>
-   match find_next_sub_pre_dtree idoms acc others with
-   | None => None
-   | Some (acc', others') => create_pre_dtree_aux others' idoms acc'
-   end
-end.
-Next Obligation. 
-  eapply find_next_sub_pre_dtree_length; eauto.
+Lemma create_predtree_aux__WF_predtree_aux: forall n, 
+  P_create_predtree_aux__WF_predtree n.
+Proof.
+  intro n.
+  apply lt_wf_rec. clear n.
+  intros n IH.
+  unfold P_create_predtree_aux__WF_predtree in *.
+  intros f idoms Hwfi pdt0 others pdt Hdis Hlen Hwf.
+  destruct others as [|l1 others]; simple_create_predtree_aux.
+    intro J. inv J; auto.
+
+    remember (find_next_sub_predtree idoms pdt0 (l1 :: others)) as R.
+    destruct R as [[acc' others']|].
+      repeat fold_sub create_predtree_aux_func ; simpl proj1_sig.
+      fold (create_predtree_aux others' idoms acc').
+      intro J. subst.
+      apply IH with (m:=length others') (f:=f) in J; auto.
+        eapply find_next_sub_predtree_length; eauto.
+        eapply find_next_sub_predtree_fresh; eauto.
+        eapply find_next_sub_predtree_wf_predtree; eauto.
+      intro J. inv J.
+Qed.
+
+Lemma create_predtree_aux__WF_predtree : forall f idoms 
+  (Hwfi: WF_idoms f idoms) pdt0 others pdt
+  (Hdis: forall l0, 
+    In l0 others -> 
+    l0 `notin` dom pdt0 `union` cdom pdt0),
+  WF_predtree f pdt0 ->
+  create_predtree_aux others idoms pdt0 = Some pdt ->
+  WF_predtree f pdt.
+Proof.
+  intros.
+  assert (J:=@create_predtree_aux__WF_predtree_aux (List.length others)).
+  unfold P_create_predtree_aux__WF_predtree in J. eauto.
 Qed.
 
 Program Fixpoint create_dtree_aux (others:set l) (res: AMap.t (set l)) 
@@ -694,46 +1451,6 @@ Next Obligation.
 Qed.
 Next Obligation. split; intros; congruence. Qed.
 
-Fixpoint dep_doms__nondep_doms_aux bd0 (res: AMap.t (Dominators.t bd0)) 
-  bd (acc: AMap.t (set l)) : AMap.t (set l) :=
-match bd with
-| nil => acc
-| l0::bd' => 
-    match AMap.get l0 res with
-    | (Dominators.mkBoundedSet dts0 _) =>
-        AMap.set l0 dts0 (dep_doms__nondep_doms_aux bd0 res bd' acc)
-    end
-end.
-
-Definition dep_doms__nondep_doms bd (res: AMap.t (Dominators.t bd)) 
-  : AMap.t (set l) :=
-dep_doms__nondep_doms_aux bd res bd (AMap.init nil).
-
-Fixpoint init_pre_dtree (idoms: list (l * l)) (root:l) (others:set l)
-  : option (PreDTree * list l) :=
-match idoms with 
-| nil => None
-| (p, ch)::idoms' => 
-    if (l_dec p root) then 
-      if (in_dec l_dec ch others) then 
-        Some ([(p, ch)], List.remove l_dec ch others)
-      else None
-    else init_pre_dtree idoms' root others
-end.
-
-Inductive WF_idoms f : list (l*l) -> Type :=
-| WF_idoms_nil : WF_idoms f nil 
-| WF_idoms_cons : forall l1 l2 idoms, 
-    imm_domination f l1 l2 -> WF_idoms f idoms ->
-    WF_idoms f ((l1,l2)::idoms)
-.
-
-Lemma WF_pre_dtree__reachable: forall f acc l1 l2,
-  WF_pre_dtree f acc ->
-  In (l1, l2) acc ->
-  reachable f l1 /\ reachable f l2.
-Admitted.
-
 Lemma find_next_child__imm_domination: forall f idoms (Hwfi: WF_idoms f idoms) 
   l1 others l2,
   find_next_child idoms l1 others = ret l2 ->
@@ -749,218 +1466,11 @@ Proof.
         inv H. auto.
 Qed.
 
-Lemma find_next_sub_pre_dtree_aux_wf_pre_dtree: 
-  forall f idoms (Hwfi: WF_idoms f idoms) acc prefix 
-    (Hwf:WF_pre_dtree f (prefix++acc)) others acc' others'
-  (Hdis: forall l0, 
-    In l0 others -> 
-    l0 `notin` dom (prefix++acc) `union` cdom (prefix++acc)),
-  find_next_sub_pre_dtree_aux idoms (prefix++acc) acc others = 
-    ret (acc', others') ->
-  WF_pre_dtree f acc'.
-Proof.
-  induction acc; simpl; intros.
-    congruence.
-
-    destruct a.
-    remember (find_next_child idoms l1 others) as R.
-    destruct R.
-      inv H.
-      apply WPDT_cons; auto.
-        apply WF_pre_dtree__reachable with (l1:=l0)(l2:=l1) in Hwf.
-          destruct Hwf; auto.
-          apply in_middle.
-        eapply find_next_child__imm_domination; eauto.
-
-        symmetry in HeqR.
-        apply find_next_child_inv in HeqR.
-        destruct HeqR as [J1 J2]. auto.
-
-        right.
-        exists l0. apply in_middle.
-
-      remember (find_next_child idoms l0 others) as R.
-      destruct R.
-        inv H.
-        apply WPDT_cons; auto.
-          apply WF_pre_dtree__reachable with (l1:=l0)(l2:=l1) in Hwf.
-            destruct Hwf; auto.
-            apply in_middle.
-          eapply find_next_child__imm_domination; eauto.
-
-          symmetry in HeqR0.
-          apply find_next_child_inv in HeqR0.
-          destruct HeqR0 as [J1 J2]. auto.
-          left. simpl_env. fsetdec.
-      rewrite_env ((prefix ++ [(l0, l1)]) ++ acc) in H.
-      apply IHacc in H; simpl_env; simpl; auto.
-Qed.
-
-Lemma find_next_sub_pre_dtree_wf_pre_dtree: 
-  forall f idoms (Hwfi: WF_idoms f idoms) pdt (Hwf:WF_pre_dtree f pdt) 
-    others pdt' others'
-  (Hdis: forall l0, 
-    In l0 others -> 
-    l0 `notin` dom pdt `union` cdom pdt),
-  find_next_sub_pre_dtree idoms pdt others = ret (pdt', others') ->
-  WF_pre_dtree f pdt'.
-Proof.
-  intros.
-  unfold find_next_sub_pre_dtree in H.
-  change pdt with (nil++pdt) in H, Hdis at 1.
-  eapply find_next_sub_pre_dtree_aux_wf_pre_dtree in H; eauto.
-Qed.
-
-Definition P_create_pre_dtree_aux__WF_pre_dtree (n:nat) :=
-  forall f idoms (Hwfi: WF_idoms f idoms) pdt0 others pdt
-  (Hdis: forall l0, 
-    In l0 others -> 
-    l0 `notin` dom pdt0 `union` cdom pdt0),
-  List.length others = n ->
-  WF_pre_dtree f pdt0 ->
-  create_pre_dtree_aux others idoms pdt0 = Some pdt ->
-  WF_pre_dtree f pdt.
-
-Require Import Program.
-
-Ltac simple_create_pre_dtree_aux :=
-  unfold create_pre_dtree_aux, create_pre_dtree_aux_func;
-  rewrite WfExtensionality.fix_sub_eq_ext;
-  repeat fold_sub create_pre_dtree_aux_func ; simpl proj1_sig;
-  simpl. 
-
-Lemma find_next_sub_pre_dtree_aux_inv: forall idoms pdt0 pdt others pdt' 
-  others',
-  find_next_sub_pre_dtree_aux idoms pdt0 pdt others = Some (pdt', others') ->
-  exists p, exists ch, 
-    pdt' = (p,ch)::pdt0 /\ others' = List.remove l_dec ch others /\
-    ((exists p', In (p', p) pdt) \/ (exists ch', In (p, ch') pdt)).
-Proof.
-  induction pdt; simpl; intros.
-    inv H.
-
-    destruct a.
-    remember (find_next_child idoms l1 others) as R.
-    destruct R.
-      inv H.
-      exists l1. exists l2. 
-      repeat split; auto.
-      left. exists l0. auto.
-
-      remember (find_next_child idoms l0 others) as R. 
-      destruct R.
-        inv H.
-        exists l0. exists l2. 
-        repeat split; auto.
-        right. exists l1. auto.
-       
-        apply IHpdt in H; auto.
-        destruct H as [p [ch [Heq1 [Heq2 [[p' J] | [ch' J]]]]]]; subst.
-          exists p. exists ch. 
-          repeat split; auto.
-          left. exists p'. auto.
-
-          exists p. exists ch. 
-          repeat split; auto.
-          right. exists ch'. auto.
-Qed.
-
-Lemma find_next_sub_pre_dtree_inv: forall idoms pdt others pdt' 
-  others',
-  find_next_sub_pre_dtree idoms pdt others = Some (pdt', others') ->
-  exists p, exists ch, 
-    pdt' = (p,ch)::pdt /\ others' = List.remove l_dec ch others /\
-    ((exists p', In (p', p) pdt) \/ (exists ch', In (p, ch') pdt)).
-Proof.
-  intros. unfold find_next_sub_pre_dtree in H.
-  apply find_next_sub_pre_dtree_aux_inv in H; auto.
-Qed.
-
-Lemma in_dom_cdom: forall p1 p2 pdt0,
-  In (p1, p2) pdt0 -> p2 `in` cdom pdt0 /\ p1 `in` dom pdt0.
-Proof.
-  induction pdt0; simpl; intros.
-    inv H.
-    destruct H as [H | H]; subst.
-      fsetdec.
-
-      destruct a.
-      apply IHpdt0 in H.
-      fsetdec.
-Qed.
-
-Lemma create_pre_dtree_aux__WF_pre_dtree_aux: forall n, 
-  P_create_pre_dtree_aux__WF_pre_dtree n.
-Proof.
-  intro n.
-  apply lt_wf_rec. clear n.
-  intros n IH.
-  unfold P_create_pre_dtree_aux__WF_pre_dtree in *.
-  intros f idoms Hwfi pdt0 others pdt Hdis Hlen Hwf.
-  destruct others as [|l1 others]; simple_create_pre_dtree_aux.
-    intro J. inv J; auto.
-
-    remember (find_next_sub_pre_dtree idoms pdt0 (l1 :: others)) as R.
-    destruct R as [[acc' others']|].
-      repeat fold_sub create_pre_dtree_aux_func ; simpl proj1_sig.
-      fold (create_pre_dtree_aux others' idoms acc').
-      intro J. subst.
-      apply IH with (m:=length others') (f:=f) in J; auto.
-        eapply find_next_sub_pre_dtree_length; eauto.
-
-        symmetry in HeqR.
-        apply find_next_sub_pre_dtree_inv in HeqR.
-        destruct HeqR as [p [ch [Heq [J1 [[p' J2] | [ch' J2]]]]]]; subst.
-          intros l0 Hin.
-          simpl.
-          assert (l0 <> ch) as Hneq.
-            assert (J':=@remove_In _ l_dec (l1 :: others) ch).
-            destruct (l_dec l0 ch); subst; auto.
-          assert (In l0 (l1::others)) as Hin'.
-            apply remove_neq_in' in Hin; auto.
-          apply Hdis in Hin'.
-          apply in_dom_cdom in J2.
-          destruct J2 as [J1 J2].
-          assert (l0 <> p) as Hneq'.
-            destruct (l_dec l0 p); subst; auto.
-          fsetdec.
- 
-          intros l0 Hin.
-          simpl.
-          assert (l0 <> ch) as Hneq.
-            assert (J':=@remove_In _ l_dec (l1 :: others) ch).
-            destruct (l_dec l0 ch); subst; auto.
-          assert (In l0 (l1::others)) as Hin'.
-            apply remove_neq_in' in Hin; auto.
-          apply Hdis in Hin'.
-          apply in_dom_cdom in J2.
-          destruct J2 as [J1 J2].
-          assert (l0 <> p) as Hneq'.
-            destruct (l_dec l0 p); subst; auto.
-          fsetdec.
-        eapply find_next_sub_pre_dtree_wf_pre_dtree; eauto.
-      intro J. inv J.
-Qed.
-
-Lemma create_pre_dtree_aux__WF_pre_dtree : forall f idoms 
-  (Hwfi: WF_idoms f idoms) pdt0 others pdt
-  (Hdis: forall l0, 
-    In l0 others -> 
-    l0 `notin` dom pdt0 `union` cdom pdt0),
-  WF_pre_dtree f pdt0 ->
-  create_pre_dtree_aux others idoms pdt0 = Some pdt ->
-  WF_pre_dtree f pdt.
-Proof.
-  intros.
-  assert (J:=@create_pre_dtree_aux__WF_pre_dtree_aux (List.length others)).
-  unfold P_create_pre_dtree_aux__WF_pre_dtree in J. eauto.
-Qed.
-
-Lemma init_pre_dtree__WF_pre_dtree : forall f root 
+Lemma init_predtree__WF_predtree : forall f root 
   (Hentry:getEntryLabel f = Some root) idoms 
   (Hwfi: WF_idoms f idoms) others pdt0 others0,
-  init_pre_dtree idoms root others = Some (pdt0, others0) ->
-  WF_pre_dtree f pdt0.
+  init_predtree idoms root others = Some (pdt0, others0) ->
+  WF_predtree f pdt0.
 Proof.
   induction idoms; simpl; intros.
     inv H.
@@ -972,8 +1482,8 @@ Proof.
       apply WPDT_entry; auto.
 Qed.
 
-Lemma init_pre_dtree__disjoint: forall root idoms others pdt0 others0,
-  init_pre_dtree idoms root others = ret (pdt0, others0) ->
+Lemma init_predtree__disjoint: forall root idoms others pdt0 others0,
+  init_predtree idoms root others = ret (pdt0, others0) ->
   ~ In root others ->
   forall l0 : atom, In l0 others0 -> l0 `notin` union (dom pdt0) (cdom pdt0).
 Proof.
@@ -1026,49 +1536,23 @@ Proof.
     apply WF_idoms_nil.
 Qed.
 
-Lemma init_create_pre_dtree_aux__WF_pre_dtree : forall f idoms pdt0 others 
+Lemma init_create_predtree_aux__WF_predtree : forall f idoms pdt0 others 
   pdt root rd,
   getEntryLabel f = Some root ->
   reachablity_analysis f = Some rd ->
   compute_idoms (dep_doms__nondep_doms (bound_fdef f) (dom_analyze f)) rd nil 
     = idoms ->
-  init_pre_dtree idoms root (List.remove eq_atom_dec root rd) 
+  init_predtree idoms root (List.remove eq_atom_dec root rd) 
     = Some (pdt0, others) ->
-  create_pre_dtree_aux others idoms pdt0 = Some pdt ->
-  WF_pre_dtree f pdt.
+  create_predtree_aux others idoms pdt0 = Some pdt ->
+  WF_predtree f pdt.
 Proof.
   intros.
   eapply compute_idoms__WF_idoms in H1; eauto.
-  eapply create_pre_dtree_aux__WF_pre_dtree in H3; eauto.
-    eapply init_pre_dtree__disjoint; eauto.
+  eapply create_predtree_aux__WF_predtree in H3; eauto.
+    eapply init_predtree__disjoint; eauto.
       apply remove_In.
-    eapply init_pre_dtree__WF_pre_dtree; eauto.
-Qed.
-
-Program Definition create_dtree (f: fdef) : option DTree :=
-match getEntryBlock f, reachablity_analysis f with
-| Some (block_intro root _ _ _), Some rd =>
-    let dt := dom_analyze f in
-    let b := bound_fdef f in
-    let idoms := compute_idoms (dep_doms__nondep_doms b dt) rd nil in
-    match init_pre_dtree idoms root (List.remove eq_atom_dec root rd) with
-    | None => None
-    | Some (pdt0, others) =>
-        match (create_pre_dtree_aux others idoms pdt0) with
-        | None => None
-        | Some pdt => 
-            tree2dtree 
-              (vertexes_of_pre_dtree pdt) (arcs_of_pre_dtree pdt)
-              (WF_pre_dtree_isa_tree f pdt _)
-        end
-    end
-| _, _ => None
-end.
-Next Obligation. 
-  eapply init_create_pre_dtree_aux__WF_pre_dtree; eauto.
-    clear - Heq_anonymous.
-    destruct f; simpl in *.
-    destruct b; simpl in *; inv Heq_anonymous. auto.
+    eapply init_predtree__WF_predtree; eauto.
 Qed.
 
 Scheme dtree_rec2 := Induction for DTree Sort Set
@@ -1170,6 +1654,7 @@ Proof.
 
     apply IHtree in H; auto.
 Qed.
+*)
 
 (*
 Definition create_dtree (f: fdef) : option DTree :=
